msIfScript.sml
@@ -36,12 +36,25 @@ val icnt_def = Define `icnt ms pa = ccnt_ ms.ic pa`;
 
 val Invic_def = Define `Invic ms = !pa. ~cdirty_ ms.ic pa`;
 
+val Invic_lem = store_thm("Invic_lem", ``
+!ms ms'. (ms.ic = ms'.ic) ==> (Invic ms <=> Invic ms')
+``,
+  RW_TAC std_ss [Invic_def]
+);
+
+
 (* lookup functions / memory views *)
 
 val dmvcl_def = Define `dmvcl ms = MVcl ms.mem`;
 val dmvca_def = Define `dmvca ms = MVca ms.dc ms.mem`;
 val dmvalt_def = Define `dmvalt ms = MValt ms.dc ms.mem`;
 val imv_def = Define `imv ms = MVca ms.ic ms.mem`;
+
+val M_dmvcl_oblg = store_thm("M_dmvcl_oblg", ``
+!ms pa c. M ms pa = dmvcl ms c pa
+``,
+  RW_TAC std_ss [M_def, dmvcl_def, MVcl_def]
+);
 
 (* transition system *)
 
@@ -113,9 +126,41 @@ val msca_DREQ_lem = store_thm("msca_DREQ_lem", ``
   ASM_REWRITE_TAC [ms_dupd_rw]
 );
 
+val msca_FREQ_lem = store_thm("msca_FREQ_lem", ``
+!ms pa ms'. (ms' = msca_trans ms (FREQ pa)) 
+    ==>
+?ca' m' dop. ((ca',m') = mtfca (ms.ic, ms.mem) dop) 
+          /\ CA dop /\ rd dop /\ (pa = PA dop)
+	  /\ (ms'.dc = ms.dc)
+          /\ (ms'.ic = ca')
+	  /\ (ms'.mem = ms.mem)
+``,
+  REWRITE_TAC [msca_trans_def] >> 
+  REPEAT STRIP_TAC >>
+  `?ca' m'. (ca',m') = mtfca (ms.ic, ms.mem) (RD pa T)` by (
+      METIS_TAC [pairTheory.pair_CASES]
+  ) >>
+  EXISTS_TAC ``ca':cache_state`` >>
+  EXISTS_TAC ``m':mem_state`` >>
+  EXISTS_TAC ``RD pa T`` >>
+  ASM_SYM_TAC mtf_pat >>
+  ASM_REWRITE_TAC [ms_iupd_rw, CA_def, rd_def, PA_def]
+);
+
+val msca_NOREQ_lem = store_thm("msca_NOREQ_lem", ``
+!ms pa ms'. (ms' = msca_trans ms NOREQ) 
+    ==>
+    (ms'.dc = ms.dc)
+ /\ (ms'.ic = ms.ic)
+ /\ (ms'.mem = ms.mem)
+``,
+  RW_TAC std_ss [msca_trans_def]
+);
+
+
 (* deriveability obligations *)
 
-val ms_cacheable_other_oblg = store_thm("ms_cacheable_other_oblg", ``
+val dc_cacheable_other_oblg = store_thm("dc_cacheable_other_oblg", ``
 !ms dop ms' pa. CA dop /\ (ms' = msca_trans ms (DREQ dop)) /\ (pa <> PA dop)
              /\ (dw ms' pa <> dw ms pa) ==> 
     ~dhit ms' pa
@@ -127,6 +172,467 @@ val ms_cacheable_other_oblg = store_thm("ms_cacheable_other_oblg", ``
   IMP_RES_TAC ca_cacheable_other_lem
 );
 
+val M_cacheable_other_oblg = store_thm("M_cacheable_other_oblg", ``
+!ms dop ms' pa. CA dop /\ (ms' = msca_trans ms (DREQ dop)) /\ (pa <> PA dop)
+                  /\ (M ms' pa <> M ms pa) ==>
+    dirty ms pa /\ (M ms' pa = dcnt ms pa)
+``,
+  REPEAT GEN_TAC >>
+  STRIP_TAC >>
+  IMP_RES_TAC msca_DREQ_lem >>
+  FULL_SIMP_TAC std_ss [dirty_def, dcnt_def, M_def] >>
+  IMP_RES_TAC mem_cacheable_other_lem >>
+  ASM_REWRITE_TAC []
+);
+
+val M_cacheable_read_oblg = store_thm("mem_cacheable_read_oblg", ``
+!ms dop ms'. CA dop /\ rd dop /\ (ms' = msca_trans ms (DREQ dop)) ==>
+    (M ms' (PA dop) = M ms (PA dop))
+``,
+  REPEAT GEN_TAC >>
+  STRIP_TAC >>
+  IMP_RES_TAC msca_DREQ_lem >>
+  FULL_SIMP_TAC std_ss [M_def] >>
+  IMP_RES_TAC mem_cacheable_read_lem
+);
+
+val dc_cacheable_read_oblg = store_thm("dc_cacheable_read_oblg", ``
+!ms dop ms'. CA dop /\ rd dop /\ (ms' = msca_trans ms (DREQ dop))
+	  /\ (dw ms' (PA dop) <> dw ms (PA dop)) 
+        ==>
+    dhit ms' (PA dop) 
+ /\ ~dirty ms' (PA dop)
+ /\ (dcnt ms' (PA dop) = M ms (PA dop))
+ /\ ~dhit ms (PA dop)
+``,
+  REPEAT GEN_TAC >>
+  STRIP_TAC >>
+  IMP_RES_TAC msca_DREQ_lem >>
+  FULL_SIMP_TAC std_ss [dhit_def, dirty_def, dw_def, dcnt_def, M_def] >>
+  IMP_RES_TAC ca_cacheable_read_lem >>
+  ASM_REWRITE_TAC []
+);
+
+val dc_cacheable_write_oblg = store_thm("dc_cacheable_write_oblg", ``
+!ms dop ms'. CA dop /\ wt dop /\ (ms' = msca_trans ms (DREQ dop))
+        ==>
+    (dirty ms' (PA dop) 
+(* WT case *)
+  \/ ~dirty ms' (PA dop) /\ (dcnt ms' (PA dop) = M ms' (PA dop)))
+``,
+  REPEAT GEN_TAC >>
+  STRIP_TAC >>
+  IMP_RES_TAC msca_DREQ_lem >>
+  FULL_SIMP_TAC std_ss [dirty_def, dcnt_def, M_def] >>
+  IMP_RES_TAC ca_cacheable_write_lem >> (
+      ASM_REWRITE_TAC []
+  )
+);
+
+val M_cacheable_not_cl_oblg = store_thm("M_cacheable_not_cl_oblg", ``
+!ms dop ms'. CA dop /\ ~cl dop /\ (ms' = msca_trans ms (DREQ dop))
+        ==>
+    ((M ms' (PA dop) = M ms (PA dop)) \/ (dcnt ms' (PA dop) = M ms' (PA dop)))
+``,
+  REPEAT GEN_TAC >>
+  STRIP_TAC >>
+  IMP_RES_TAC msca_DREQ_lem >>
+  FULL_SIMP_TAC std_ss [dcnt_def, M_def] >>
+  IMP_RES_TAC mem_cacheable_not_cl_lem >> (
+      ASM_REWRITE_TAC []
+  )
+);
+
+(* uncacheable accesses *)
+
+val ms_uncacheable_unchanged_oblg = store_thm("ms_uncacheable_unchanged_oblg", ``
+!ms dop ms'. ~CA dop /\ ~wt dop /\ (ms' = msca_trans ms (DREQ dop))
+        ==>
+    (dw ms' = dw ms) /\ (M ms' = M ms)
+``,
+  REPEAT GEN_TAC >>
+  STRIP_TAC >>
+  IMP_RES_TAC msca_DREQ_lem >>
+  RW_TAC std_ss [FUN_EQ_THM] >> (
+      FULL_SIMP_TAC std_ss [dw_def, M_def] >>
+      IMP_RES_TAC uncacheable_unchanged_lem >> 
+      ASM_REWRITE_TAC []
+  )
+);
+
+val M_uncacheable_unchanged_oblg = store_thm("M_uncacheable_unchanged_oblg", ``
+!ms dop ms'. ~CA dop /\ ~wt dop /\ (ms' = msca_trans ms (DREQ dop))
+        ==>
+    (M ms' (PA dop) = M ms (PA dop))
+``,
+  REPEAT GEN_TAC >>
+  STRIP_TAC >>
+  IMP_RES_TAC msca_DREQ_lem >>
+  FULL_SIMP_TAC std_ss [M_def] >>
+  IMP_RES_TAC mem_uncacheable_unchanged_lem
+);
+
+val M_uncacheable_write_oblg = store_thm("M_uncacheable_write_oblg", ``
+!ms dop ms'. wt dop /\ (ms' = msca_trans ms (DREQ dop))
+	  /\ (M ms' (PA dop) <> M ms (PA dop))
+        ==>
+    (~CA dop \/ (dcnt ms' (PA dop) = M ms' (PA dop)))
+``,
+  REPEAT GEN_TAC >>
+  STRIP_TAC >>
+  IMP_RES_TAC msca_DREQ_lem >>
+  FULL_SIMP_TAC std_ss [dcnt_def, M_def] >>
+  IMP_RES_TAC mem_uncacheable_write_lem >> (
+      ASM_REWRITE_TAC []
+  )
+);
+
+(* Data Coherency *)
+
+val dcoh_def = Define `dcoh ms pa = coh ms.dc ms.mem pa`;
+val dCoh_def = Define `dCoh ms (Rs:padr set) = Coh ms.dc ms.mem Rs`;
+
+val dCoh_alt_oblg = store_thm("dCoh_alt_oblg", ``
+!ms Rs. dCoh ms Rs 
+            <=> 
+        !pa. pa IN Rs ==> ((dmvca ms) T pa = (dmvalt ms) T pa)
+``,
+  REWRITE_TAC [dCoh_def, dmvca_def, dmvalt_def, Coh_alt_lem]
+);
+
+val dcoh_write_oblg = store_thm("dcoh_write_oblg", ``
+!ms dop ms'. CA dop /\ wt dop /\ (ms' = msca_trans ms (DREQ dop))
+        ==>
+   dcoh ms' (PA dop)
+``,
+  REPEAT GEN_TAC >>
+  STRIP_TAC >>
+  IMP_RES_TAC msca_DREQ_lem >>
+  FULL_SIMP_TAC std_ss [dcoh_def] >>
+  IMP_RES_TAC coh_write_lem
+);
+
+val dcoh_ca_trans_oblg = store_thm("dcoh_ca_trans_oblg", ``
+!ms dop ms' pa. CA dop /\ dcoh ms pa /\ (ms' = msca_trans ms (DREQ dop))
+        ==>
+    dcoh ms' pa
+``,
+  REPEAT GEN_TAC >>
+  STRIP_TAC >>
+  IMP_RES_TAC msca_DREQ_lem >>
+  FULL_SIMP_TAC std_ss [dcoh_def] >>
+  IMP_RES_TAC coh_ca_trans_lem
+);
+
+val dc_unchanged_oblg = store_thm("dc_unchanged_oblg", ``
+!ms dop ms'. CA dop /\ ~wt dop /\ dcoh ms (PA dop)
+	  /\ (ms' = msca_trans ms (DREQ dop))
+        ==>
+    (dmvca ms' T (PA dop) = dmvca ms T (PA dop))
+``,
+  REPEAT GEN_TAC >>
+  STRIP_TAC >>
+  IMP_RES_TAC msca_DREQ_lem >>
+  FULL_SIMP_TAC std_ss [dcoh_def, dmvca_def] >>
+  IMP_RES_TAC ca_unchanged_lem
+);
+
+
+val dc_other_unchanged_oblg = store_thm("dc_other_unchanged_oblg", ``
+!ms dop ms' pa. dcoh ms pa /\ (pa <> PA dop)
+	     /\ (ms' = msca_trans ms (DREQ dop))
+        ==>
+    (dmvca ms' T pa = dmvca ms T pa)
+``,
+  REPEAT GEN_TAC >>
+  STRIP_TAC >>
+  IMP_RES_TAC msca_DREQ_lem >>
+  FULL_SIMP_TAC std_ss [dcoh_def, dmvca_def] >>
+  IMP_RES_TAC ca_other_unchanged_lem
+);
+
+(* instruction cache *)
+
+val Invic_fetch_lem = store_thm("Invic_fetch_lem", ``
+!ms pa ms'. Invic ms /\ (ms' = msca_trans ms (FREQ pa)) 
+         ==> 
+    Invic ms'
+``,
+  REPEAT STRIP_TAC >>
+  FULL_SIMP_TAC std_ss [Invic_def] >>
+  IMP_RES_TAC msca_FREQ_lem >>
+  STRIP_TAC >>
+  PAT_X_ASSUM ``!pa. X`` ( fn thm => ASSUME_TAC ( SPEC ``pa':padr`` thm ) ) >>
+  `~wt dop` by ( METIS_TAC [dop_cases_lem2] ) >>
+  Cases_on `pa' = PA dop` 
+  >| [(* PA dop *)
+      RW_TAC std_ss [] >>
+      Cases_on `(msca_trans ms (FREQ (PA dop))).ic (PA dop) = ms.ic (PA dop)`
+      >| [(* cache hit *)
+	  METIS_TAC [cdirty_lem]
+	  ,
+	  (* cache miss *)
+	  IMP_RES_TAC ca_cacheable_read_lem
+	 ]
+      ,
+      (* other pa' *)
+      Cases_on `ca' pa' = ms.ic pa'` 
+      >| [(* unchanged *)
+	  METIS_TAC [cdirty_lem]
+	  ,
+	  (* eviction *)
+	  RW_TAC std_ss [] >>
+	  IMP_RES_TAC ca_cacheable_other_lem >>
+	  IMP_RES_TAC not_chit_not_cdirty_lem
+	 ]
+     ]	  	  
+);
+
+val Invic_preserve_oblg = store_thm("Invic_preserve_oblg", ``
+!ms req ms'. Invic ms /\ (ms' = msca_trans ms req) ==> Invic ms'
+``,
+  REPEAT STRIP_TAC >>
+  Cases_on `req` 
+  >| [(* DREQ *)
+      IMP_RES_TAC msca_DREQ_lem >>
+      IMP_RES_TAC Invic_lem
+      ,
+      (* FREQ *)
+      IMP_RES_TAC Invic_fetch_lem
+      ,
+      (* NOREQ *)
+      IMP_RES_TAC msca_NOREQ_lem >>
+      IMP_RES_TAC Invic_lem
+     ]
+);
+
+(* Instruction Cache Coherency *)
+
+val icoh_def = Define `icoh ms pa = 
+(ihit ms pa ==> (icnt ms pa = M ms pa)) /\ ~dirty ms pa`;
+val dCoh_def = Define `iCoh ms (Rs:padr set) = !pa. pa IN Rs ==> icoh ms pa`;
+
+val icoh_lem = store_thm("icoh_lem", ``
+!ms pa. Invic ms ==> 
+    (icoh ms pa <=> coh ms.ic ms.mem pa /\ ~cdirty_ ms.dc pa)
+``,
+  RW_TAC std_ss [Invic_def, icoh_def, coh_def, ihit_def, icnt_def, 
+		 M_def, dirty_def] >>
+  REWRITE_TAC [IMP_DISJ_THM]
+);
+
+val icoh_fetch_lem = store_thm("icoh_fetch_lem", ``
+!ms req ms' pa. icoh ms pa /\ (ms' = msca_trans ms (FREQ pa))
+        ==>
+    icoh ms' pa
+``,
+  REPEAT STRIP_TAC >>
+  IMP_RES_TAC msca_FREQ_lem >>
+  Cases_on `ca' pa = ms.ic pa`
+  >| [(* hit *)
+      FULL_SIMP_TAC std_ss [icoh_def, ihit_def, icnt_def, M_def] >>
+      STRIP_TAC 
+      >| [(* icoh *)
+	  RW_TAC std_ss [] >>
+	  IMP_RES_TAC chit_lem >>
+	  IMP_RES_TAC ccnt_lem >>
+	  RW_TAC std_ss []
+	  ,
+	  (* not dirty in dc *)
+	  FULL_SIMP_TAC std_ss [dirty_def] >>
+	  RW_TAC std_ss [cdirty_lem]
+	 ]
+      ,
+      (* miss *)
+      RW_TAC std_ss [] >>
+      IMP_RES_TAC ca_cacheable_read_lem >>
+      RW_TAC std_ss [icoh_def, ihit_def, icnt_def, M_def] >>
+      FULL_SIMP_TAC std_ss [icoh_def, dirty_def] >>
+      RW_TAC std_ss [cdirty_lem]
+     ]
+);
+
+val icoh_fetch_other_lem = store_thm("icoh_fetch_other_lem", ``
+!ms req ms' pa pa'. icoh ms pa' /\ (ms' = msca_trans ms (FREQ pa)) /\ pa' <> pa
+        ==>
+    icoh ms' pa'
+``,
+  REPEAT STRIP_TAC >>
+  IMP_RES_TAC msca_FREQ_lem >>
+  Cases_on `ca' pa' = ms.ic pa'`
+  >| [(* hit *)
+      FULL_SIMP_TAC std_ss [icoh_def, ihit_def, icnt_def, M_def] >>
+      STRIP_TAC 
+      >| [(* icoh *)
+	  RW_TAC std_ss [] >>
+	  IMP_RES_TAC chit_lem >>
+	  IMP_RES_TAC ccnt_lem >>
+	  RW_TAC std_ss []
+	  ,
+	  (* not dirty in dc *)
+	  FULL_SIMP_TAC std_ss [dirty_def] >>
+	  RW_TAC std_ss [cdirty_lem]
+	 ]
+      ,
+      (* miss *)
+      RW_TAC std_ss [] >>
+      IMP_RES_TAC ca_cacheable_other_lem >>
+      RW_TAC std_ss [icoh_def, ihit_def, icnt_def, M_def] >>
+      FULL_SIMP_TAC std_ss [icoh_def, dirty_def] >>
+      RW_TAC std_ss [cdirty_lem]
+     ]
+);
+
+val icoh_not_write_lem = store_thm("icoh_not_write_lem", ``
+!ms dop ms' pa. icoh ms pa /\ ~wt dop /\ (ms' = msca_trans ms (DREQ dop))
+        ==>
+    icoh ms' pa
+``,
+  REPEAT STRIP_TAC >>
+  IMP_RES_TAC msca_DREQ_lem >>
+  Cases_on `CA dop`
+  >| [(* cacheable *)
+      FULL_SIMP_TAC std_ss [icoh_def, ihit_def, icnt_def, M_def, dirty_def] >>
+      IMP_RES_TAC ca_cacheable_mem >>
+      PAT_X_ASSUM ``!pa. X`` ( fn thm => ASSUME_TAC ( SPEC ``pa:padr`` thm ) ) >>
+      REV_FULL_SIMP_TAC std_ss [] >>
+      Cases_on `ca' pa = ms.dc pa`
+      >| [(* unchanged *)
+	  METIS_TAC [cdirty_lem]
+	  ,
+	  (* changed *)
+	  Cases_on `pa = PA dop`
+	  >| [(* PA dop *)
+	      FULL_SIMP_TAC std_ss [not_wt_lem]
+	      >| [(* read miss *)
+		  RW_TAC std_ss [] >>
+		  IMP_RES_TAC ca_cacheable_read_lem
+		  ,
+		  (* clean *)
+		  IMP_RES_TAC ca_cacheable_cl_lem >>
+	          PAT_X_ASSUM ``!pa. X`` ( 
+		      fn thm => ASSUME_TAC ( SPEC ``pa:padr`` thm ) 
+		  ) >>
+		  REV_FULL_SIMP_TAC std_ss [] >>
+		  IMP_RES_TAC not_chit_not_cdirty_lem >>
+		  RW_TAC std_ss []
+		 ]
+	      ,
+	      (* other pa *)
+	      IMP_RES_TAC ca_cacheable_other_lem >>
+	      IMP_RES_TAC not_chit_not_cdirty_lem 
+	     ]
+	 ]
+      ,
+      (* uncacheable *)
+      IMP_RES_TAC uncacheable_unchanged_lem >>
+      FULL_SIMP_TAC std_ss [icoh_def, ihit_def, icnt_def, M_def, dirty_def]
+     ]
+);
+
+val icoh_write_other_lem = store_thm("icoh_write_other_lem", ``
+!ms dop ms' pa. icoh ms pa /\ wt dop /\ (pa <> PA dop)
+	     /\ (ms' = msca_trans ms (DREQ dop))
+        ==>
+    icoh ms' pa
+``,
+  REPEAT STRIP_TAC >>
+  IMP_RES_TAC msca_DREQ_lem >>
+  Cases_on `CA dop`
+  >| [(* cacheable *)
+      FULL_SIMP_TAC std_ss [icoh_def, ihit_def, icnt_def, M_def, dirty_def] >>
+      IMP_RES_TAC ca_cacheable_mem >>
+      PAT_X_ASSUM ``!pa. X`` ( fn thm => ASSUME_TAC ( SPEC ``pa:padr`` thm ) ) >>
+      REV_FULL_SIMP_TAC std_ss [] >>
+      Cases_on `ca' pa = ms.dc pa`
+      >| [(* unchanged *)
+	  METIS_TAC [cdirty_lem]
+	  ,
+	  (* changed *)
+	  IMP_RES_TAC ca_cacheable_other_lem >>
+	  IMP_RES_TAC not_chit_not_cdirty_lem 
+	 ]
+      ,
+      (* uncacheable *)
+      IMP_RES_TAC ca_uncacheable >>
+      IMP_RES_TAC cl_other_unchanged_lem >>
+      FULL_SIMP_TAC std_ss [icoh_def, ihit_def, icnt_def, M_def, dirty_def] >>
+      RW_TAC std_ss []
+     ]
+);
+
+
+val icoh_preserve_oblg = store_thm("icoh_preserve_oblg", ``
+!ms req ms' pa. icoh ms pa /\ (ms' = msca_trans ms req)
+	     /\ (Wreq req ==> (pa <> Adr req))
+        ==>
+    icoh ms' pa
+``,
+  REPEAT STRIP_TAC >>
+  Cases_on `req`
+  >| [(* DREQ *)
+      Cases_on `Wreq (DREQ d)`
+      >| [(* write *)
+	  RES_TAC >>
+	  `wt d` by ( FULL_SIMP_TAC std_ss [Wreq_def] ) >>
+	  FULL_SIMP_TAC std_ss [Adr_def] >>
+	  IMP_RES_TAC icoh_write_other_lem >>
+	  RW_TAC std_ss []
+	  ,
+	  (* not write *)
+	  `~wt d` by ( FULL_SIMP_TAC std_ss [Wreq_def] ) >>
+	  IMP_RES_TAC icoh_not_write_lem 
+	 ]
+      ,
+      (* FREQ *)
+      Cases_on `pa = p`
+      >| [(* fetched pa *)
+	  FULL_SIMP_TAC std_ss [] >>
+	  IMP_RES_TAC icoh_fetch_lem >>
+	  RW_TAC std_ss []
+	  ,
+	  (* other address *)
+	  IMP_RES_TAC icoh_fetch_other_lem
+	 ]
+      ,
+      (* NOREQ *)
+      IMP_RES_TAC msca_NOREQ_lem >>
+      FULL_SIMP_TAC std_ss [icoh_def, ihit_def, icnt_def, M_def, dirty_def]
+     ]
+);
+
+val imv_dmv_oblg = store_thm("imv_dmv_oblg", ``
+!ms pa. icoh ms pa /\ dcoh ms pa ==> (imv ms T pa = dmvca ms T pa)
+``,
+  RW_TAC std_ss [icoh_def, ihit_def, icnt_def, imv_def, M_def,
+		 dcoh_def, dirty_def, dmvca_def, MVca_def] >>
+  IMP_RES_TAC coh_clean_lem >>
+  RW_TAC std_ss []
+);
+
+val imv_dmvcl_oblg = store_thm("imv_dmv_oblg", ``
+!ms pa c. icoh ms pa ==> (imv ms T pa = dmvcl ms c pa)
+``,
+  RW_TAC std_ss [icoh_def, ihit_def, icnt_def, imv_def, M_def,
+		 dirty_def, dmvcl_def, MVcl_def, MVca_def]
+);
+
+
+(* val Invic_imv_oblg = store_thm("Invic_imv_oblg", `` *)
+(* !ms req ms' pa. Invic ms /\ icoh ms pa /\ (ms' = msca_trans ms req) *)
+(* 	     /\ (Wreq req ==> (pa <> Adr req)) *)
+(*         ==> *)
+(*     (imv ms' T pa = imv ms T pa) *)
+(* ``, *)
+(*   REPEAT STRIP_TAC >> *)
+(*   Cases_on `req` *)
+(*   >| [(* DREQ *) *)
+(*       , *)
+(*       (* FREQ *) *)
+(*       , *)
+(*       (* NOREQ *) *)
+(*      ] *)
+(* ); *)
 
 (*********** finish ************)
 
